src/Pipeline.v
@@ -20,7 +20,7 @@ Require Import riscv.RiscvBitWidths.
 Require Import compiler.NameWithEq.
 Require Import riscv.encode.Encode.
 Require Import riscv.AxiomaticRiscv.
-
+Require Import riscv.proofs.DecodeEncode.
 
 Section Pipeline.
 
@@ -38,6 +38,8 @@ Section Pipeline.
   (* assumes generic translate and raiseException functions *)
   Context {RVS: @RiscvState (OState RiscvMachine) (word wXLEN) _ _ RVM}.  
 
+  Existing Instance FlatToRiscv.State_is_RegisterFile.
+  
   Context {RVAX: @AxiomaticRiscv Bw state FlatToRiscv.State_is_RegisterFile (mem wXLEN) _ RVM}.
 
   Definition var := Register.
@@ -58,41 +60,180 @@ Section Pipeline.
   Definition evalL(fuel: nat)(insts: list Instruction)(initial: RiscvMachine): RiscvMachine :=
     execState (run fuel) (putProgram (map (fun i => ZToWord 32 (encode i)) insts) initial).
 
+  Lemma wXLEN_32: 32 <= wXLEN.
+  Proof.
+    clear. unfold wXLEN, bitwidth. destruct Bw; omega.
+  Qed.
+
+  Lemma wXLEN_cases: wXLEN = 32 \/ wXLEN = 64.
+  Proof.
+    clear. unfold wXLEN, bitwidth. destruct Bw; omega.
+  Qed.
+
+  Arguments mult: simpl never.
+
+  (* TODO put into Memory.v *)
+  Lemma store_word_list_preserves_memSize_aux: forall sz (m: mem wXLEN) a l,
+      length l = sz ->
+      Memory.memSize (Memory.store_word_list l a m) = Memory.memSize m.
+  Proof.
+    induction sz; intros; subst; destruct l; simpl in *; try congruence.
+    inversions H.
+    rewrite IHsz by reflexivity.
+    apply Memory.storeWord_preserves_memSize.
+  Qed.
+
+  Lemma store_word_list_preserves_memSize: forall (m: mem wXLEN) l a,
+      Memory.memSize (Memory.store_word_list l a m) = Memory.memSize m.
+  Proof.
+    intros. eapply store_word_list_preserves_memSize_aux. reflexivity.
+  Qed.
+
+  Lemma loadWord_before_store_word_list: forall sz (m: mem wXLEN) l (a1 a2: word wXLEN),
+      length l = sz ->
+      #a1 + 4 <= #a2 ->
+      #a2 + 4 * sz <= (Memory.memSize m) ->
+      Memory.valid_addr a1 4 (Memory.memSize m) ->
+      Memory.valid_addr a2 4 (Memory.memSize m) ->
+      Memory.loadWord (Memory.store_word_list l a2 m) a1  = Memory.loadWord m a1.
+  Proof.
+    induction sz; intros; subst; destruct l; simpl in *; try congruence.
+    inversions H.
+    pose proof (Memory.memSize_bound m).
+    rewrite IHsz.
+    - apply Memory.loadStoreWord_ne; try assumption.
+      intro C. subst. omega.
+    - reflexivity.
+    - pose proof FlatToRiscv.pow2_wXLEN_4.
+      unfold Memory.valid_addr in *. intuition idtac.
+      rewrite wordToNat_wplus'; rewrite wordToNat_natToWord_idempotent'; try omega.
+      (* TODO similar to containsProgram stuff *)
+      admit.
+    - admit.
+    - rewrite Memory.storeWord_preserves_memSize. assumption.
+    - rewrite Memory.storeWord_preserves_memSize. (* TODO *) admit.
+  Admitted.
+
+  Lemma loadWord_store_word_list: forall i (m: mem wXLEN) l a,
+      0 <= i < length l ->
+      Memory.valid_addr a 4 (Memory.memSize m) ->
+      Memory.loadWord (Memory.store_word_list l a m) (a ^+ $(4 * i))  = nth i l $0.
+  Proof.
+    induction i; intros; destruct l; simpl in *.
+    - exfalso. omega.
+    - erewrite loadWord_before_store_word_list.
+      + apply Memory.loadStoreWord_eq.
+        * assumption.
+        * (* TODO make FlatToRiscv.solve_word_eq available *) admit.
+      + reflexivity.
+      + admit.
+      + (* TODO needs more hyps *) admit.
+      + rewrite Memory.storeWord_preserves_memSize. admit.
+      + admit.
+    - exfalso. omega.
+    - replace (a ^+ $ (4 * S i)) with ((a ^+ $4) ^+ $(4 * i)) by admit.
+      rewrite IHi.
+      + reflexivity.
+      + omega.
+      + rewrite Memory.storeWord_preserves_memSize. admit.
+  Admitted.
+
+  Lemma putProgram_containsProgram: forall p (initial: RiscvMachine),
+    4 * (length p) <= Memory.memSize initial.(machineMem) ->
+    FlatToRiscv.containsProgram
+      (putProgram (map (fun i : Instruction => ZToWord 32 (encode i)) p) initial).(machineMem) p $0.
+  Proof.  
+    intros. unfold FlatToRiscv.containsProgram, putProgram.
+    intros.
+    destruct initial as [[regs pc0 eh] m].
+    rewrite roundTrip_0. simpl in *. split.
+    - rewrite store_word_list_preserves_memSize. assumption.
+    - intros.
+      unfold FlatToRiscv.ldInst.
+      rewrite loadWord_store_word_list.
+      + remember (fun i0 : Instruction => ZToWord 32 (encode i0)) as f.
+        replace (natToWord 32 0) with (f (InvalidInstruction 0)) by (subst; reflexivity).
+        rewrite map_nth.
+        erewrite nth_error_nth by eassumption.
+        subst f.
+        rewrite wordToZ_ZToWord.
+        * replace RV_wXLEN_IM with RV64IMA by admit. (* TODO *)
+          apply decode_encode; [|reflexivity].
+          (* TODO argue that inst was emitted by compiler and therefore respects imm bounds *)
+          admit.
+        * (* TODO argue that inst was emitted by compiler and therefore is 32 bits *)
+          admit.
+      + assert (i < length p). {
+          apply nth_error_Some. intro. congruence.
+        }
+        rewrite map_length.
+        omega.
+      + unfold Memory.valid_addr.
+        rewrite roundTrip_0. simpl.
+        destruct p; simpl in *.
+        * exfalso. eapply FlatToRiscv.nth_error_nil_Some. eassumption.
+        * omega.
+  Admitted.
+
+  (* We could also say something about the memory, but then the statement becomes more complex.
+     And note that the register we look at could contain any value loaded from the memory. *)
   Lemma exprImp2Riscv_correct: forall sH initialL instsL fuelH finalH initialMemH finalMemH,
-    ExprImp.stmt_size sH * 64 < pow2 wXLEN ->
+    ExprImp.stmt_size sH < 2 ^ 14 ->
     exprImp2Riscv sH = instsL ->
+    4 * length instsL <= Memory.memSize initialL.(machineMem) ->
     evalH fuelH empty initialMemH sH = Some (finalH, finalMemH) ->
+    FlatToRiscv.mem_inaccessible initialMemH 0 (4 * length instsL) ->
     exists fuelL,
       forall resVar res,
       get finalH resVar = Some res ->
       getReg (evalL fuelL instsL initialL).(core).(registers) resVar = res.
   Proof.
-    introv B C EvH.
+    introv B C MB EvH Ina.
     unfold exprImp2Riscv in C.
     destruct_one_match_hyp.
     unfold evalH in EvH.
-  Admitted.
-  (* TODO first finish FlatToRiscv.compile_stmt_correct
     pose proof flattenStmt_correct as P.
-    specialize (P fuelH sH s finalH).
+    specialize (P fuelH sH s initialMemH finalH finalMemH).
     destruct P as [fuelM [finalM [EvM GM]]].
     - unfold ExprImp2FlatImp. rewrite E. reflexivity.
     - unfold evalH. apply EvH.
     - pose proof  FlatToRiscv.compile_stmt_correct as P.
-      specialize P with (2 := C).
-      specialize P with (2 := EvM).
-      specialize (P initialL).
-      destruct P as [fuelL P].
-      + pose proof @flattenStmt_size as D1.
+      specialize P with (imemStart := $0).
+      let r := eval unfold evalL in (evalL 0 instsL initialL) in
+          match r with
+          | execState _ ?x => specialize P with (initialL := x)
+          end.
+      edestruct P as [fuelL [P1 P2]].
+      + admit. (* TODO translate_id *)
+      + admit. (* TODO translate_id *)
+      + eassumption.
+      + unfold FlatToRiscv.stmt_not_too_big.
+        pose proof @flattenStmt_size as D1.
         specialize D1 with (1 := E).
         clear -B D1.
+        change 20 with (16 + 4).
+        rewrite Nat.pow_add_r.
+        apply Nat.mul_lt_mono_pos_r; [ simpl; omega | ].
+        change 16 with (2 + 14).
+        rewrite Nat.pow_add_r.
+        change (2 ^ 2) with 4.
         omega.
-      + exists fuelL.
-        introv G.
-        apply P.
-        apply GM.
-        apply G.
-  Qed.
-  *)
+      + admit. (* TODO valid_registers *)
+      + rewrite roundTrip_0. reflexivity.
+      + eassumption.
+      + admit. (* TODO containsMem! *)
+      + apply putProgram_containsProgram.
+        assumption.
+      + reflexivity.
+      + simpl. rewrite wplus_unit. reflexivity.
+      + rewrite roundTrip_0. assumption.
+      + exists fuelL. intros.
+        clear P.
+        unfold getReg, FlatToRiscv.State_is_RegisterFile.
+        unfold StateCalculus.extends in P1.
+        unfold evalL.
+        erewrite P1; try reflexivity.
+        apply GM. exact H.
+  Admitted.
 
 End Pipeline.
